Regex/Regex.lean
@@ -96,7 +96,7 @@ theorem String.Pos.sub_lt_sub_left {k m n : String.Pos} (h1 : k < m) (h2 : k < n
 
 theorem String.Pos.sizeof_lt_of_lt {a b : String.Pos} (h : a < b) : sizeOf a < sizeOf b := by
   have sizeOf_string_pos {s : String.Pos} : sizeOf (s) = 1 + sizeOf s.byteIdx := rfl
-  apply String.Pos.lt_def.mp at h
+  simp [String.Pos.lt_def.mp] at h
   rw [sizeOf_string_pos, sizeOf_string_pos, sizeOf_nat, sizeOf_nat]
   omega
 
